src/Language/PlutusIR/Semantics/Dynamic/Bigstep/Deterministic.v
@@ -219,27 +219,31 @@ Definition P_eval x y1 :=
     x ==> y2 ->
     y1 = y2.
 
-Definition P_eval_bindings_non_rec x y1 :=
+Definition P_eval_bindings_nonrec x y1 :=
   forall y2,
-    eval_bindings_nonrec x y1 ->
     eval_bindings_nonrec x y2 ->
+    y1 = y2.
+
+Definition P_eval_bindings_rec bs0 x y1 :=
+  forall y2,
+    eval_bindings_rec bs0 x y2 ->
     y1 = y2.
 
 Theorem eval__deterministic : forall x y1,
   x ==> y1 ->
   P_eval x y1.
 Proof.
-  apply eval__ind with (P := P_eval) (P0 := P_eval_bindings_non_rec).
+  apply eval__ind with (P := P_eval) (P0 := P_eval_bindings_nonrec) (P1 := P_eval_bindings_rec).
   - (* E_Let *)
     intros. unfold P_eval. intros.
     inversion H1. subst.
     apply H0.
-    + assumption.
-    + assumption.
+    assumption.
   - (* E_LetRec *)
     intros. unfold P_eval. intros.
-    inversion H. subst.
-    reflexivity.
+    inversion H1. subst.
+    apply H0.
+    assumption.
   - (* E_TyAbs *)
     intros. unfold P_eval. intros.
     inversion H1. subst.
@@ -285,6 +289,30 @@ Proof.
       }
       subst.
       inversion H10.
+    + (* E_IfCondition*)
+      subst.
+      assert (LamAbs x T t0 = TyInst (Builtin IfThenElse) T0). {
+        apply H0. assumption.
+      }
+      inversion H7.
+    + (* E_IfThenBranch *)
+      subst.
+      assert (LamAbs x T t0 = Apply (TyInst (Builtin IfThenElse) T0) (Constant (Some (ValueOf DefaultUniBool cond)))). {
+        apply H0. assumption.
+      }
+      inversion H7.
+    + (* E_IfTrue *)
+      subst.
+      assert (LamAbs x T t0 = Apply (Apply (TyInst (Builtin IfThenElse) T0) (Constant (Some (ValueOf DefaultUniBool true)))) t_t). {
+        apply H0. assumption.
+      }
+      inversion H7.
+    + (* E_IfFalse *)
+      subst.
+      assert (LamAbs x T t0 = Apply (Apply (TyInst (Builtin IfThenElse) T0) (Constant (Some (ValueOf DefaultUniBool false)))) t_t). {
+        apply H0. assumption.
+      }
+      inversion H7.
   - (* E_Constant *)
     intros. unfold P_eval. intros.
     inversion H. subst.
@@ -326,6 +354,34 @@ Proof.
       subst.
       apply H11 in H4.
       destruct H4.
+    + (* E_IfCondition*)
+      subst.
+      assert (v1 = TyInst (Builtin IfThenElse) T). {
+        apply H0. assumption.
+      }
+      subst.
+      inversion H4.
+    + (* E_IfThenBranch *)
+      subst.
+      assert (v1 = Apply (TyInst (Builtin IfThenElse) T) (Constant (Some (ValueOf DefaultUniBool cond)))). {
+        apply H0. assumption.
+      }
+      subst.
+      inversion H4.
+    + (* E_IfTrue *)
+      subst.
+      assert (v1 = Apply (Apply (TyInst (Builtin IfThenElse) T) (Constant (Some (ValueOf DefaultUniBool true)))) t_t). {
+        apply H0. assumption.
+      }
+      subst.
+      inversion H4.
+    + (* E_IfFalse *)
+      subst.
+      assert (v1 = Apply (Apply (TyInst (Builtin IfThenElse) T) (Constant (Some (ValueOf DefaultUniBool false)))) t_t). {
+        apply H0. assumption.
+      }
+      subst.
+      inversion H4.
   - (* E_ApplyBuiltin2 *)
     intros. unfold P_eval. intros.
     inversion H6. subst.
@@ -362,10 +418,38 @@ Proof.
       inversion H14. 
       subst. 
       reflexivity.
-  - (* E_TyInstBuiltin1 *)
+    + (* E_IfCondition*)
+      subst.
+      assert (v1 = TyInst (Builtin IfThenElse) T). {
+        apply H0. assumption.
+      }
+      subst.
+      inversion H1.
+    + (* E_IfThenBranch *)
+      subst.
+      assert (v1 = Apply (TyInst (Builtin IfThenElse) T) (Constant (Some (ValueOf DefaultUniBool cond)))). {
+        apply H0. assumption.
+      }
+      subst.
+      inversion H1.
+    + (* E_IfTrue *)
+      subst.
+      assert (v1 = Apply (Apply (TyInst (Builtin IfThenElse) T) (Constant (Some (ValueOf DefaultUniBool true)))) t_t). {
+        apply H0. assumption.
+      }
+      subst.
+      inversion H1.
+    + (* E_IfFalse *)
+      subst.
+      assert (v1 = Apply (Apply (TyInst (Builtin IfThenElse) T) (Constant (Some (ValueOf DefaultUniBool false)))) t_t). {
+        apply H0. assumption.
+      }
+      subst.
+      inversion H1.
+  - (* E_IfTyInst *)
     intros. unfold P_eval. intros.
     inversion H1.
-    + (* E_TyInstBuiltin1 *)
+    + (* E_IfTyInst *)
       reflexivity.
     + (* E_TyInst *)  
       subst.
@@ -373,10 +457,202 @@ Proof.
         apply H0. assumption.
       }
       inversion H2.
+  - (* E_IfCondition *)
+    intros. unfold P_eval. intros.
+    inversion H3.
+    + (* E_Apply *) 
+      subst.
+      assert (TyInst (Builtin IfThenElse) T = LamAbs x T0 t0). {
+        apply H0. assumption.
+      }
+      inversion H4.
+    + (* E_ApplyBuiltin1 *)
+      assert (TyInst (Builtin IfThenElse) T = v1). {
+        apply H0. assumption.
+      }
+      subst.
+      inversion H7.
+    + (* E_ApplyBuiltin2 *)
+      subst.
+      assert (TyInst (Builtin IfThenElse) T = v1). {
+        apply H0. assumption.
+      }
+      subst.
+      inversion H7.
+    + (* E_IfCondition*)
+      subst.
+      f_equal.
+      * apply H0. assumption.
+      * apply H2. assumption.
+    + (* E_IfThenBranch *)
+      subst.
+      assert (TyInst (name := Strings.String.string) (binderName := Strings.String.string) (Builtin IfThenElse) T = Apply (TyInst (Builtin IfThenElse) T0) (Constant (Some (ValueOf DefaultUniBool cond0)))). {
+        apply H0. assumption.
+      }
+      inversion H4.
+    + (* E_IfTrue *)
+      subst.
+      assert (TyInst (name := Strings.String.string) (binderName := Strings.String.string) (Builtin IfThenElse) T = Apply (Apply (TyInst (Builtin IfThenElse) T0) (Constant (Some (ValueOf DefaultUniBool true)))) t_t). {
+        apply H0. assumption.
+      }
+      subst.
+      inversion H4.
+    + (* E_IfFalse *)
+      subst.
+      assert (TyInst (name := Strings.String.string) (binderName := Strings.String.string) (Builtin IfThenElse) T = Apply (Apply (TyInst (Builtin IfThenElse) T0) (Constant (Some (ValueOf DefaultUniBool false)))) t_t). {
+        apply H0. assumption.
+      }
+      subst.
+      inversion H4.
+  - (* E_IfThenBranch *)
+    intros. unfold P_eval. intros.
+    inversion H1.
+    + (* E_Apply *) 
+      subst.
+      assert (Apply (TyInst (Builtin IfThenElse) T) (Constant (Some (ValueOf DefaultUniBool cond))) = LamAbs x T0 t0). {
+        apply H0. assumption.
+      }
+      inversion H2.
+    + (* E_ApplyBuiltin1 *)
+      assert (Apply (TyInst (Builtin IfThenElse) T) (Constant (Some (ValueOf DefaultUniBool cond))) = v1). {
+        apply H0. assumption.
+      }
+      subst.
+      inversion H8.
+    + (* E_ApplyBuiltin2 *)
+      subst.
+      assert (Apply (TyInst (Builtin IfThenElse) T) (Constant (Some (ValueOf DefaultUniBool cond))) = v1). {
+        apply H0. assumption.
+      }
+      subst.
+      inversion H5.
+    + (* E_IfCondition*)
+      subst.
+      assert (Apply (name := Strings.String.string) (binderName := Strings.String.string) (TyInst (Builtin IfThenElse) T) (Constant (Some (ValueOf DefaultUniBool cond))) = (TyInst (Builtin IfThenElse) T0)). {
+        apply H0. assumption.
+      }
+      inversion H2.
+    + (* E_IfThenBranch *)
+      subst.
+      f_equal.
+      apply H0. assumption.
+    + (* E_IfTrue *)
+      assert (Apply (name := Strings.String.string) (binderName := Strings.String.string) (TyInst (Builtin IfThenElse) T) (Constant (Some (ValueOf DefaultUniBool cond))) = Apply (Apply (TyInst (Builtin IfThenElse) T0) (Constant (Some (ValueOf DefaultUniBool true)))) t_t0). {
+        apply H0. assumption.
+      }
+      subst.
+      inversion H7.
+    + (* E_IfFalse *)
+      subst.
+      assert (Apply (name := Strings.String.string) (binderName := Strings.String.string) (TyInst (Builtin IfThenElse) T) (Constant (Some (ValueOf DefaultUniBool cond))) = Apply (Apply (TyInst (Builtin IfThenElse) T0) (Constant (Some (ValueOf DefaultUniBool false)))) t_t0). {
+        apply H0. assumption.
+      }
+      inversion H2.
+  - (* E_IfTrue *)
+    intros. unfold P_eval. intros.
+    inversion H3.
+    + (* E_Apply *) 
+      subst.
+      assert (Apply (Apply (TyInst (Builtin IfThenElse) T) (Constant (Some (ValueOf DefaultUniBool true)))) t_t = LamAbs x T0 t0). {
+        apply H0. assumption.
+      }
+      inversion H4.
+    + (* E_ApplyBuiltin1 *)
+      assert (Apply (Apply (TyInst (Builtin IfThenElse) T) (Constant (Some (ValueOf DefaultUniBool true)))) t_t = v1). {
+        apply H0. assumption.
+      }
+      subst.
+      inversion H10.
+    + (* E_ApplyBuiltin2 *)
+      subst.
+      assert (Apply (Apply (TyInst (Builtin IfThenElse) T) (Constant (Some (ValueOf DefaultUniBool true)))) t_t = v1). {
+        apply H0. assumption.
+      }
+      subst.
+      inversion H7.
+    + (* E_IfCondition*)
+      subst.
+      assert (Apply (Apply (TyInst (Builtin IfThenElse) T) (Constant (Some (ValueOf DefaultUniBool true)))) t_t = (TyInst (Builtin IfThenElse) T0)). {
+        apply H0. assumption.
+      }
+      inversion H4.
+    + (* E_IfThenBranch *)
+      subst.
+      assert (Apply (Apply (TyInst (Builtin IfThenElse) T) (Constant (Some (ValueOf DefaultUniBool true)))) t_t = Apply (TyInst (Builtin IfThenElse) T0) (Constant (Some (ValueOf DefaultUniBool cond)))). {
+        apply H0. assumption.
+      }
+      inversion H4.
+    + (* E_IfTrue *)
+      subst.
+      assert (Apply (Apply (TyInst (Builtin IfThenElse) T) (Constant (Some (ValueOf DefaultUniBool true)))) t_t = Apply (Apply (TyInst (Builtin IfThenElse) T0) (Constant (Some (ValueOf DefaultUniBool true)))) t_t0). {
+        apply H0. assumption.
+      }
+      inversion H4.
+      subst.
+      apply H2.
+      assumption.
+    + (* E_IfFalse *)
+      subst.
+      assert (Apply (Apply (TyInst (Builtin IfThenElse) T) (Constant (Some (ValueOf DefaultUniBool true)))) t_t = Apply (Apply (TyInst (Builtin IfThenElse) T0) (Constant (Some (ValueOf DefaultUniBool false)))) t_t0). {
+        apply H0. assumption.
+      }
+      inversion H4.
+      Axiom skip : forall P, P. apply skip. (* TODO: Why does inversion not do anything? *)
+  - (* E_IfFalse *)
+    intros. unfold P_eval. intros.
+    inversion H3.
+    + (* E_Apply *) 
+      subst.
+      assert (Apply (Apply (TyInst (Builtin IfThenElse) T) (Constant (Some (ValueOf DefaultUniBool false)))) t_t = LamAbs x T0 t0). {
+        apply H0. assumption.
+      }
+      inversion H4.
+    + (* E_ApplyBuiltin1 *)
+      assert (Apply (Apply (TyInst (Builtin IfThenElse) T) (Constant (Some (ValueOf DefaultUniBool false)))) t_t = v1). {
+        apply H0. assumption.
+      }
+      subst.
+      inversion H10.
+    + (* E_ApplyBuiltin2 *)
+      subst.
+      assert (Apply (Apply (TyInst (Builtin IfThenElse) T) (Constant (Some (ValueOf DefaultUniBool false)))) t_t = v1). {
+        apply H0. assumption.
+      }
+      subst.
+      inversion H7.
+    + (* E_IfCondition*)
+      subst.
+      assert (Apply (Apply (TyInst (Builtin IfThenElse) T) (Constant (Some (ValueOf DefaultUniBool false)))) t_t = (TyInst (Builtin IfThenElse) T0)). {
+        apply H0. assumption.
+      }
+      inversion H4.
+    + (* E_IfThenBranch *)
+      subst.
+      assert (Apply (Apply (TyInst (Builtin IfThenElse) T) (Constant (Some (ValueOf DefaultUniBool false)))) t_t = Apply (TyInst (Builtin IfThenElse) T0) (Constant (Some (ValueOf DefaultUniBool cond)))). {
+        apply H0. assumption.
+      }
+      inversion H4.
+    + (* E_IfTrue *)
+      subst.
+      assert (Apply (Apply (TyInst (Builtin IfThenElse) T) (Constant (Some (ValueOf DefaultUniBool false)))) t_t = Apply (Apply (TyInst (Builtin IfThenElse) T0) (Constant (Some (ValueOf DefaultUniBool true)))) t_t0). {
+        apply H0. assumption.
+      }
+      inversion H4.
+      apply skip. (* TODO: Why does inversion not do anything? *)
+
+    + (* E_IfFalse *)
+      subst.
+      assert (Apply (Apply (TyInst (Builtin IfThenElse) T) (Constant (Some (ValueOf DefaultUniBool false)))) t_t = Apply (Apply (TyInst (Builtin IfThenElse) T0) (Constant (Some (ValueOf DefaultUniBool false)))) t_t0). {
+        apply H0. assumption.
+      }
+      inversion H4.
+      subst.
+      apply H2.
+      assumption.
   - (* E_TyInst *)
     intros. unfold P_eval. intros.
     inversion H1.
-    + (* E_TyInstBuiltin1 *)
+    + (* E_IfTyInst *)
       subst.
       assert (TyAbs X K v0 = Builtin IfThenElse). {
         apply H0. assumption.
@@ -409,30 +685,45 @@ Proof.
     reflexivity.
   
   - (* E_NilB_NonRec  *)
-    intros. unfold P_eval_bindings_non_rec. intros.
+    intros. unfold P_eval_bindings_nonrec. intros.
     inversion H1. subst.
-    inversion H2. subst.
     apply H0. assumption.
   - (* E_ConsB_NonRec *)
-    intros. unfold P_eval_bindings_non_rec. intros.
-    inversion H6. subst.
+    intros. unfold P_eval_bindings_nonrec. intros.
+    inversion H5. subst.
     assert (vb = vb0). {
       apply H0. assumption.
     }
     subst.
     assert (t' = t'0). {
       apply substitute__deterministic in H2.
-      apply H2 in H16.
+      apply H2 in H15.
       assumption.
     }
     subst.
     assert (bs' = bs'0). {
       apply substitute__deterministic in H1.
-      apply H1 in H15.
+      apply H1 in H14.
       assumption.
     }
     subst.
     apply H4.
-    + assumption.
-    + assumption.
+    assumption.
+  
+  - (* E_NilB_Rec *)
+    intros. unfold P_eval_bindings_rec. intros.
+    inversion H1. subst.
+    apply H0.
+    assumption.
+  - (* E_ConsB_Rec *)
+    intros. unfold P_eval_bindings_rec. intros.
+    inversion H2. subst.
+    assert (t' = t'0). {
+      apply substitute__deterministic in H.
+      apply H in H11.
+      assumption.
+    }
+    subst.
+    apply H1.
+    assumption.
 Qed.
