src/Language/PlutusIR/Semantics/Dynamic/Bigstep/EvalToValue.v
@@ -3,14 +3,16 @@ Import NamedTerm.
 Require Import PlutusCert.Language.PlutusIR.Semantics.Dynamic.Bigstep.
 
 Definition P_eval (t v : Term) := value v.
-Definition P_eval_bindings_non_rec (t v : Term) := value v.
+Definition P_eval_bindings_nonrec (t v : Term) := value v.
+Definition P_eval_bindings_rec (bs0 : list Binding) (t v : Term) := value v.
 
 Lemma eval_to_value : forall t v,
     t ==> v -> value v.
 Proof.
-  eapply eval__ind with (P := P_eval) (P0 := P_eval_bindings_non_rec); try (intros; unfold P_eval; unfold P_eval_bindings_non_rec).
+  eapply eval__ind with (P := P_eval) (P0 := P_eval_bindings_nonrec) (P1 := P_eval_bindings_rec); 
+    try (intros; unfold P_eval; unfold P_eval_bindings_nonrec; unfold P_eval_bindings_rec).
   - assumption.
-  - Axiom skip : forall P, P. apply skip. (* TODO *)
+  - assumption.
   - apply V_TyAbs. assumption.
   - apply V_LamAbs.
   - assumption.
@@ -36,18 +38,6 @@ Proof.
           destruct v; inversion H5.
           apply V_Constant.
         }
-        destruct v1_1_1; inversion H5.
-        destruct d; inversion H5.
-        destruct v1_1_2; inversion H5.
-        destruct s; inversion H5.
-        destruct u; inversion H5.
-        destruct v; inversion H5.
-        destruct u.
-        - subst.
-          inversion H1. subst.
-          assumption.
-        - subst.
-          apply H3.
       }
       destruct d; inversion H5; 
         try solve [
@@ -70,11 +60,17 @@ Proof.
         destruct v; inversion H5;
         apply V_Constant
       ].
-  - apply V_Builtin. apply V_Builtin1_WithTyInst. apply le_S. apply le_S. apply le_n.
-  - inversion H0; subst. assumption. inversion H1.
+  - apply V_IfTyInst.
+  - apply V_IfCondition.
+  - apply V_IfThenBranch.
+  - assumption.
+  - assumption.
+  - inversion H0; subst; auto. inversion H1. 
   - apply V_Error.
   - apply V_IWrap. apply H0.
   - inversion H0; subst. inversion H1. assumption.
+  - assumption.
+  - assumption.
   - assumption.
   - assumption.
 Qed.
