src/Language/PlutusIR/Semantics/TypeSafety/SubstitutionPreservesTyping.v
@@ -71,20 +71,162 @@ Proof.
 Qed.
 
 
-Lemma binds_binds_bound_vars : forall a x U v,
-  List.In x (term_vars_bound_by_binding a) ->
-  emptyContext |-+ v : U ->
-  lookupT (binds a) x = Datatypes.Some U.
-Proof. Admitted.
+Lemma binds_binds_bound_vars : forall a x,
+    List.In x (term_vars_bound_by_binding a) ->
+    exists U, lookupT (binds a) x = Datatypes.Some U.
+Proof.
+  intros.
+  destruct a.
+  - simpl.
+    destruct (getName v =? x) eqn:Heqb.
+    + apply eqb_eq in Heqb as Heq.
+      subst.
+      exists (getTy v).
+      apply update_eq.
+    + apply eqb_neq in Heqb as Hneq.
+      simpl in H.
+      destruct v.
+      simpl in H.
+      destruct H.
+      * apply Hneq in H.
+        destruct H.
+      * destruct H.
+  - simpl in H.
+    destruct t.
+    inversion H.
+  - simpl.
+Admitted.
+
+Lemma mapbinds_binds_bound_vars : forall bs x,
+  List.In x (term_vars_bound_by_bindings bs) ->
+  exists U, lookupT (flatten (List.map binds bs)) x = Datatypes.Some U.
+Proof.
+  induction bs.
+  - intros.
+    inversion H.
+  - intros.
+    unfold term_vars_bound_by_bindings in H.
+    simpl in H.
+    apply List.in_app_or in H.
+    destruct H.
+    + simpl.
+      unfold flatten.
+      simpl.
+      rewrite concat_append.
+      simpl. 
+      destruct (lookupT (Named.concat (List.rev (List.map binds bs))) x).
+      * exists t.
+        reflexivity.
+      * destruct (lookupT (binds a) x) eqn:Hlookup.
+        -- exists t.
+           reflexivity.
+        -- apply binds_binds_bound_vars in H.
+           destruct H. 
+           rewrite H in Hlookup.
+           inversion Hlookup.
+    + simpl.
+      unfold flatten.
+      simpl.
+      rewrite concat_append.
+      simpl.
+      destruct (lookupT (Named.concat (List.rev (List.map binds bs))) x) eqn:Hlookup.
+      * exists t.
+        reflexivity.
+      * apply IHbs in H.
+        destruct H.
+        unfold flatten in H.
+        rewrite H in Hlookup.
+        inversion Hlookup.
+Qed.
 
 Lemma binds_unbinds_unbound_vars : forall a x,
-  ~(List.In x (term_vars_bound_by_binding a)) ->
-  lookupT (binds a) x = None.
-Proof. Admitted.
+    ~(List.In x (term_vars_bound_by_binding a)) ->
+    lookupT (binds a) x = None.
+Proof.
+  intros.
+  destruct a.
+  - simpl.
+    destruct (getName v =? x) eqn:Heqb.
+    + apply eqb_eq in Heqb as Heq.
+      subst.
+      destruct v.
+      exfalso.
+      apply H.
+      simpl.
+      left.
+      reflexivity.
+    + apply eqb_neq in Heqb as Hneq.
+      apply update_neq.
+      assumption.
+  - reflexivity.
+  - simpl.
+    destruct d.
+    simpl.
+    destruct (s =? x) eqn:Heqb.
+    + apply eqb_eq in Heqb as Heq.
+      subst.
+      exfalso.
+      apply H.
+      simpl.
+      destruct t.
+      simpl.
+      left.
+      reflexivity.
+    + apply eqb_neq in Heqb as Hneq.
+      rewrite update_neq; auto.
+      destruct  (lookupT
+      (List.fold_right Named.append emptyContext
+         (List.map
+            (fun x0 : binderTyname * Ty => fst x0 |T-> snd x0; emptyContext)
+            (List.map (constrBind (Datatype t l s l0)) l0))) x) eqn:E.
+      * exfalso.
+        apply H.
+        simpl.
+        destruct t.
+        simpl.
+        right.
+Admitted.
+
+Lemma mapbinds_unbinds_unbound_vars : forall bs x,
+    ~(List.In x (term_vars_bound_by_bindings bs)) ->
+    lookupT (flatten (List.map binds bs)) x = None.
+Proof.
+  induction bs.
+  - intros.
+    reflexivity.
+  - intros.
+    simpl.
+    unfold flatten.
+    simpl.
+    rewrite concat_append.
+    simpl.
+    destruct (lookupT (Named.concat (List.rev (List.map binds bs))) x) eqn:Hlookup.
+    + rewrite IHbs in Hlookup.
+      * symmetry in Hlookup.
+        assumption.
+      * intros Hcon.
+        apply H.
+        unfold term_vars_bound_by_bindings.
+        simpl.
+        apply List.in_or_app.
+        right.
+        assumption.
+    + destruct (lookupT (binds a) x) eqn:Hlookup'.
+      * rewrite binds_unbinds_unbound_vars in Hlookup'.
+        -- auto.
+        -- intros Hcon.
+           apply H.
+           unfold term_vars_bound_by_bindings.
+           simpl.
+           apply List.in_or_app.
+           left.
+           assumption.
+      * reflexivity.
+Qed.
 
 Theorem context_invariance_T__has_kind : forall T ctx_T ctx_K K ctx_T',
-  (ctx_T, ctx_K) |-* T : K ->
-  (ctx_T', ctx_K) |-* T : K.
+    (ctx_T, ctx_K) |-* T : K ->
+    (ctx_T', ctx_K) |-* T : K.
 Proof.
   induction T.
   - intros.
@@ -157,7 +299,15 @@ Definition P_Bindings_NonRec (bs : list Binding) :=
     substitute_bindings_nonrec x v bs bs' ->
     ctx |-oks_nr bs' /\ List.map binds bs = List.map binds bs'.
 
-Lemma e : forall bs, P_Bindings_NonRec bs.
+Definition P_Bindings_Rec (bs : list Binding) :=
+  forall ctx x U v bs',
+    extendT x U ctx |-oks_r bs ->
+    emptyContext |-+ v : U ->
+    Util.ForallT P_Binding bs ->
+    substitute_bindings_rec x v bs bs' ->
+    ctx |-oks_r bs' /\ List.map binds bs = List.map binds bs'.
+
+Lemma P_Bindings_NonRec__holds_definitionally : forall bs, P_Bindings_NonRec bs.
 Proof.
   induction bs.
   - unfold P_Bindings_NonRec.
@@ -182,8 +332,9 @@ Proof.
            inversion H. subst.
            destruct (X _ _ _ _ _ H5 H0 H8).
            rewrite <- H3.
+           apply binds_binds_bound_vars in H6.
+           destruct H6.
            erewrite append_extendT_shadow in H7; eauto.
-           eapply binds_binds_bound_vars; eauto.
       * simpl.
         apply Util.ForallT_hd in X.
         inversion H. subst.
@@ -225,7 +376,42 @@ Proof.
         -- eapply Util.ForallT_tl. eauto.
 Qed.
 
-Axiom skip : forall P, P.
+Lemma P_Bindings_Rec__holds_definitionally : forall bs, P_Bindings_Rec bs.
+Proof.
+  induction bs.
+  - unfold P_Bindings_Rec.
+    intros.
+    inversion H1. subst.
+    auto with typing.
+  - unfold P_Bindings_Rec.
+    intros.
+    inversion H1.
+    + subst.
+      split.
+      * apply W_ConsB_Rec.
+        -- apply Util.ForallT_hd in X.
+           unfold P_Binding in X.
+           eapply X.
+           ++ inversion H. subst.
+              apply H5.
+           ++ apply H0.
+           ++ assumption.
+        -- apply Util.ForallT_tl in X.
+           eapply IHbs; eauto.
+           inversion H. subst.
+           auto.
+      * simpl.
+        inversion H. subst.
+        f_equal.
+        -- assert (binds a = binds b'). {
+            apply Util.ForallT_hd in X.
+             eapply X; eauto.
+           }
+           subst.
+           auto.
+        -- apply Util.ForallT_tl in X.
+           eapply IHbs; eauto.
+Qed.
 
 Lemma substitution_preserves_typing : forall t, P_Term t.
 Proof.
@@ -235,27 +421,85 @@ Proof.
     + subst.
       eapply T_Let.
       * reflexivity.
-      * eapply e.
+      * eapply P_Bindings_NonRec__holds_definitionally.
         -- inversion H0. subst.
             eauto.
         -- eauto.
         -- eauto.
         -- eauto.
       * inversion H0. subst.
-        apply skip.
+        assert (List.map binds bs = List.map binds bs'). {
+          eapply P_Bindings_NonRec__holds_definitionally.
+          -- inversion H0. subst.
+             eauto.
+          -- eauto.
+          -- eauto.
+          -- eauto.
+        }
+        rewrite <- H3.
+        apply mapbinds_binds_bound_vars in H9.
+        destruct H9. 
+        erewrite append_extendT_shadow in H11.
+        -- assumption.
+        -- apply H4.
     + subst.
       inversion H0. subst.
       eapply T_Let.
       * reflexivity.
-      * eapply e.
-        -- inversion H0. subst.
-           eauto.
+      * eapply P_Bindings_NonRec__holds_definitionally.
         -- eauto.
         -- eauto.
         -- eauto.
-      * apply skip.
-    + apply skip.
-    + apply skip.
+        -- eauto.
+      * assert (List.map binds bs = List.map binds bs'). {
+          eapply P_Bindings_NonRec__holds_definitionally.
+          -- eauto.
+          -- eauto.
+          -- eauto.
+          -- eauto.
+        }
+        rewrite <- H3.
+        apply mapbinds_unbinds_unbound_vars in H8 as H13.
+        rewrite append_extendT_permute in H12; auto.
+        eapply H; eauto.
+    + subst.
+      inversion H0. subst.
+      eapply T_LetRec.
+      * reflexivity.
+      * apply mapbinds_binds_bound_vars in H9 as H11. 
+        destruct H11.
+        erewrite append_extendT_shadow in H7; eauto.
+      * apply mapbinds_binds_bound_vars in H9 as H11. 
+        destruct H11.
+        erewrite append_extendT_shadow in H10; eauto.
+    + subst.
+      inversion H0. subst.
+      eapply T_LetRec.
+      * reflexivity.
+      * apply mapbinds_unbinds_unbound_vars in H8 as H13.
+        rewrite append_extendT_permute in H12; auto.
+        rewrite append_extendT_permute in H7; auto.
+        assert (List.map binds bs = List.map binds bs'). {
+          eapply P_Bindings_Rec__holds_definitionally.
+          -- eauto.
+          -- eauto.
+          -- eauto.
+          -- eauto.
+        }
+        rewrite <- H3.
+        eapply (P_Bindings_Rec__holds_definitionally bs); eauto.
+      * apply mapbinds_unbinds_unbound_vars in H8 as H13.
+        rewrite append_extendT_permute in H12; auto.
+        rewrite append_extendT_permute in H7; auto.
+        assert (List.map binds bs = List.map binds bs'). {
+          eapply P_Bindings_Rec__holds_definitionally.
+          -- eauto.
+          -- eauto.
+          -- eauto.
+          -- eauto.
+        }
+        rewrite <- H3.
+        eapply H; eauto.
   - intros. autounfold. intros.
     inversion H1.
     + subst.
