src/Language/PlutusIR/Semantics/Dynamic/Bigstep/Examples/AddInteger.v
@@ -1,0 +1,60 @@
+Require Import PlutusCert.Language.PlutusIR.
+Import NamedTerm.
+Require Import PlutusCert.Language.PlutusIR.Semantics.Dynamic.Bigstep.
+
+Require Import Coq.ZArith.BinInt.
+Local Open Scope Z_scope.
+Require Import Coq.Lists.List.
+Import ListNotations.
+Require Import Coq.Strings.String.
+Local Open Scope string_scope.
+
+
+
+Definition Ty_int : Ty := Ty_Builtin (Some (TypeIn DefaultUniInteger)).
+Definition int_to_int : Ty := Ty_Fun Ty_int Ty_int.
+
+Example test_addInteger : forall x,
+  Apply (LamAbs x int_to_int (Apply (Var x) (constInt 17))) (Apply (Builtin AddInteger) (constInt 3))
+  ==> constInt 20.
+Proof.
+  intros.
+  eapply E_Apply.
+  - apply E_LamAbs.
+  - eapply E_ApplyBuiltin1.
+    + apply E_Builtin.
+    + apply V_Builtin0.
+      simpl.
+      apply le_S.
+      apply le_n.
+    + apply E_Constant.
+    + apply V_Builtin1.
+      * simpl.
+        apply le_n.
+      * apply V_Constant.
+  - apply S_Apply.
+    + apply S_Var1.
+    + apply S_Constant.
+  - eapply E_ApplyBuiltin2.
+    + eapply E_ApplyBuiltin1.
+      * apply E_Builtin.
+      * apply V_Builtin0.
+        simpl.
+        apply le_S.
+        apply le_n.
+      * apply E_Constant.
+      * apply V_Builtin1.
+        -- simpl.
+           apply le_n.
+        -- apply V_Constant.
+    + apply V_Builtin1.
+      -- apply le_n.
+      -- apply V_Constant.
+    + apply E_Constant.
+    + intros Hcon.
+      inversion Hcon. subst.
+      simpl in H2.
+      apply PeanoNat.Nat.lt_irrefl in H2.
+      inversion H2. 
+    +  reflexivity.
+Qed.
