src/Language/PlutusIR/Semantics/Dynamic/Bigstep/Examples/Factorial.v
@@ -1,0 +1,433 @@
+Require Import PlutusCert.Language.PlutusIR.
+Import NamedTerm.
+Require Import PlutusCert.Language.PlutusIR.Semantics.Dynamic.Bigstep.
+
+Require Import Coq.ZArith.BinInt.
+Local Open Scope Z_scope.
+Require Import Coq.Lists.List.
+Import ListNotations.
+Require Import Coq.Strings.String.
+Local Open Scope string_scope.
+
+Definition fact_term (n : Z) : Term :=
+  Let 
+    Rec
+    [ TermBind 
+        Strict 
+        (VarDecl 
+          "fact" 
+          (Ty_Fun 
+            (Ty_Builtin (Some (TypeIn DefaultUniInteger))) 
+            (Ty_Builtin (Some (TypeIn DefaultUniInteger)))
+          )
+        ) 
+        (LamAbs 
+          "x" 
+          (Ty_Builtin (Some (TypeIn DefaultUniInteger)))
+          (Apply
+            (Apply
+              (Apply
+                (TyInst
+                  (Builtin IfThenElse)
+                  (Ty_Builtin (Some (TypeIn DefaultUniInteger)))  
+                )
+                (Apply
+                  (Apply
+                    (Builtin EqInteger)
+                    (Var "x")
+                  )
+                  (Constant (Some (ValueOf DefaultUniInteger 0)))
+                )
+              )
+              (Constant (Some (ValueOf DefaultUniInteger 1)))
+            )
+            (Apply
+              (Apply
+                (Builtin MultiplyInteger)
+                (Var "x")
+              )
+              (Apply
+                (Var "fact")
+                (Apply
+                  (Apply
+                    (Builtin SubtractInteger)
+                    (Var "x")
+                  )
+                  (Constant (Some (ValueOf DefaultUniInteger 1)))
+                )
+              )
+            )
+          )
+        )
+    ] 
+    (Apply
+      (Var "fact")
+      (Constant (Some (ValueOf DefaultUniInteger n)))  
+    ).
+
+Ltac invert_contra := let Hcon := fresh "Hcon" in intros Hcon; inversion Hcon.
+Ltac destruct_invert_contra := let Hcon := fresh "Hcon" in intros Hcon; destruct Hcon as [Hcon | Hcon]; try solve [inversion Hcon || destruct Hcon].
+Ltac solve_substitute := repeat (econstructor || eauto || invert_contra || destruct_invert_contra).
+Ltac solve_value_builtin := repeat econstructor.
+
+Example fact_term_evaluates : 
+  fact_term 2 ==> Constant (Some (ValueOf DefaultUniInteger 2)).
+Proof with eauto.
+  apply E_LetRec.
+  eapply E_ConsB_Rec. {
+    apply S_Apply. 
+    - apply S_Var1.
+    - apply S_Constant.
+  }
+  apply E_NilB_Rec.
+  eapply E_Apply. {
+    eapply E_LetRec.
+    eapply E_ConsB_Rec. {
+      apply S_LamAbs2.
+      - intros Hcon.
+        inversion Hcon.
+      - apply S_Apply.
+        + apply S_Apply.
+          * apply S_Apply. 
+            -- apply S_TyInst.
+               apply S_Builtin.
+            -- apply S_Apply. 
+               ++ apply S_Apply.
+                  ** apply S_Builtin.
+                  ** apply S_Var2. 
+                     intros Hcon.
+                     inversion Hcon.
+               ++ apply S_Constant.
+          * apply S_Constant.
+        + apply S_Apply. 
+          * apply S_Apply.
+            -- apply S_Builtin.
+            -- apply S_Var2.
+               intros Hcon.
+               inversion Hcon.
+          * apply S_Apply.
+            -- apply S_Var1.
+            -- apply S_Apply.
+               ++ apply S_Apply.
+                  ** apply S_Builtin.
+                  ** apply S_Var2.
+                     intros Hcon.
+                     inversion Hcon.
+               ++ apply S_Constant.
+    }
+    apply E_NilB_Rec.
+    apply E_LamAbs.
+  } {
+    apply E_Constant.
+  } {
+    apply S_Apply.
+    - apply S_Apply.
+      + apply S_Apply.
+        * apply S_TyInst.
+          apply S_Builtin.
+        * apply S_Apply.
+          -- apply S_Apply.
+             ++ apply S_Builtin.
+             ++ apply S_Var1.
+          -- apply S_Constant.
+      + apply S_Constant.
+    - apply S_Apply. 
+      + apply S_Apply.
+        * apply S_Builtin.
+        * apply S_Var1.
+      + apply S_Apply.
+        * apply S_LetRec2.
+          -- intros Hcon.
+             simpl in Hcon.
+             destruct Hcon.
+             ++ inversion H.
+             ++ destruct H.
+          -- apply S_ConsB_Rec.
+             ++ apply S_TermBind.
+                apply S_LamAbs1.
+             ++ apply S_NilB_Rec.
+          -- apply S_LamAbs1.
+        * apply S_Apply.
+          -- apply S_Apply.
+             ++ apply S_Builtin.
+             ++ apply S_Var1.
+          -- apply S_Constant.
+  }
+  eapply E_IfFalse. { 
+    eapply E_IfThenBranch. {
+      eapply E_IfCondition. {
+        eapply E_IfTyInst. {
+          apply E_Builtin.
+        }
+      } {
+        eapply E_ApplyBuiltin2. {
+          eapply E_ApplyBuiltin1. {
+            apply E_Builtin.
+          } {
+            eapply V_Builtin0.
+            apply PeanoNat.Nat.lt_0_succ.
+          } {
+            apply E_Constant.
+          } {
+            apply V_Builtin1.
+            - apply le_n.
+            - apply V_Constant.
+          }
+        } {
+          eapply V_Builtin1.
+          - apply le_n.
+          - apply V_Constant.
+        } {
+          apply E_Constant.
+        } {
+          intros Hcon.
+          inversion Hcon. subst.
+          apply PeanoNat.Nat.lt_irrefl in H2.
+          destruct H2.
+        } 
+        reflexivity.
+      }
+    }
+  } 
+  eapply E_ApplyBuiltin2. {
+    eapply E_ApplyBuiltin1. {
+      apply E_Builtin.
+    } {
+      eapply V_Builtin0.
+      apply PeanoNat.Nat.lt_0_succ.
+    } {
+      eapply E_Constant.
+    } {
+      eapply V_Builtin1. {
+        apply le_n.
+      } {
+        eapply V_Constant.
+      }
+    }
+  } {
+    eapply V_Builtin1. {
+      apply le_n.
+    } {
+      eapply V_Constant.
+    }
+  } {
+    eapply E_Apply. {
+      eapply E_LetRec. {
+        eapply E_ConsB_Rec. {
+          solve_substitute.
+        } {
+          eapply E_NilB_Rec.
+          eapply E_LamAbs.
+        }
+      }
+    } {
+      eapply E_ApplyBuiltin2. {
+        eapply E_ApplyBuiltin1. {
+          eapply E_Builtin.
+        } {
+          eapply V_Builtin0.
+          apply PeanoNat.Nat.lt_0_succ.
+        } {
+          eapply E_Constant.
+        } {
+          eapply V_Builtin1. {
+            eapply le_n.
+          } {
+            eapply V_Constant.
+          }
+        }
+      } {
+        eapply V_Builtin1. {
+          eapply le_n.
+        } {
+          eapply V_Constant.
+        }
+      } {
+        eapply E_Constant.
+      } {
+        intros Hcon.
+        inversion Hcon. subst.
+        apply PeanoNat.Nat.lt_irrefl in H2.
+        destruct H2.
+      } {
+        reflexivity.
+      }
+    } {
+      eapply S_Apply. {
+        eapply S_Apply. {
+          eapply S_Apply. {
+            solve_substitute.
+          } {
+            solve_substitute.
+          }
+        } {
+          solve_substitute.
+        }
+      } {
+        eapply S_Apply. {
+          solve_substitute.
+        } {
+          eapply S_Apply. {
+            eapply S_LetRec2. {
+              destruct_invert_contra.
+            } {
+              solve_substitute.
+            } {
+              solve_substitute.
+            }
+          } {
+            solve_substitute.
+          }
+        }
+      }
+    } {
+      eapply E_IfFalse. {
+        eapply E_IfThenBranch. {
+          eapply E_IfCondition. {
+            eapply E_IfTyInst.
+            eapply E_Builtin.
+          } {
+            eapply E_ApplyBuiltin2. {
+              eapply E_ApplyBuiltin1. {
+                eapply E_Builtin.
+              } {
+                eapply V_Builtin0.
+                apply PeanoNat.Nat.lt_0_succ.
+              } {
+                eapply E_Constant.
+              } {
+                eapply V_Builtin1. {
+                  eapply le_n.
+                } {
+                  eapply V_Constant.
+                }
+              }
+            } {
+              eapply V_Builtin1. {
+                eapply le_n.
+              } {
+                eapply V_Constant.
+              }
+            } {
+              eapply E_Constant.
+            } {
+              invert_contra.
+              apply PeanoNat.Nat.lt_irrefl in H2.
+              destruct H2.
+            } {
+              reflexivity.
+            }
+          }
+        }
+      } {
+        eapply E_ApplyBuiltin2. {
+          eapply E_ApplyBuiltin1. {
+            eapply E_Builtin.
+          } {
+            solve_value_builtin.
+          } {
+            eapply E_Constant.
+          } {
+            solve_value_builtin.
+          }
+        } {
+          solve_value_builtin.
+        } {
+          eapply E_Apply. {
+            eapply E_LetRec. {
+              eapply E_ConsB_Rec. {
+                solve_substitute.
+              } {
+                eapply E_NilB_Rec.
+                eapply E_LamAbs.
+              }
+            }
+          } {
+            eapply E_ApplyBuiltin2. {
+              eapply E_ApplyBuiltin1. {
+                eapply E_Builtin.
+              } {
+                solve_value_builtin.
+              } {
+                eapply E_Constant.
+              } {
+                solve_value_builtin.
+              }
+            } {
+              solve_value_builtin.
+            } {
+              eapply E_Constant.
+            } {
+              invert_contra.
+              apply PeanoNat.Nat.lt_irrefl in H2.
+              destruct H2.
+            } {
+              reflexivity.
+            }
+          } {
+            eapply S_Apply. {
+              solve_substitute.
+            } {
+              eapply S_Apply... {
+                eapply S_Apply... {
+                  eapply S_LetRec2. {
+                    destruct_invert_contra.
+                  } {
+                    solve_substitute.
+                  } {
+                    solve_substitute.
+                  }
+                }
+              }
+            }
+          } {
+            eapply E_IfTrue. {
+              eapply E_IfThenBranch. {
+                eapply E_IfCondition. {
+                  eapply E_IfTyInst. 
+                  eapply E_Builtin.
+                } {
+                  eapply E_ApplyBuiltin2. {
+                    eapply E_ApplyBuiltin1. {
+                      eapply E_Builtin.
+                    } {
+                      solve_substitute.
+                    } {
+                      eapply E_Constant.
+                    } {
+                      solve_value_builtin.
+                    }
+                  } {
+                    solve_value_builtin.
+                  } {
+                    eapply E_Constant.
+                  } {
+                    invert_contra.
+                    apply PeanoNat.Nat.lt_irrefl in H2.
+                    destruct H2.
+                  } {
+                    reflexivity.
+                  }
+                }
+              }
+            } {
+              apply E_Constant.
+            }
+          }
+        } {
+          invert_contra.
+          apply PeanoNat.Nat.lt_irrefl in H2.
+          destruct H2.
+        } {
+          reflexivity.
+        }
+      }
+    }
+  } {
+    invert_contra.
+    apply PeanoNat.Nat.lt_irrefl in H2.
+    destruct H2.
+  } {
+    reflexivity.
+  }
+Qed.
