src/Language/PlutusIR/Semantics/Dynamic/Bigstep/Examples/IfThenElse.v
@@ -1,0 +1,42 @@
+Require Import PlutusCert.Language.PlutusIR.
+Import NamedTerm.
+Require Import PlutusCert.Language.PlutusIR.Semantics.Dynamic.Bigstep.
+
+Require Import Coq.ZArith.BinInt.
+Local Open Scope Z_scope.
+Require Import Coq.Lists.List.
+Import ListNotations.
+Require Import Coq.Strings.String.
+Local Open Scope string_scope.
+
+
+Definition Ty_int : Ty := Ty_Builtin (Some (TypeIn DefaultUniInteger)).
+Definition int_and_int_to_int : Ty := Ty_Fun Ty_int (Ty_Fun Ty_int Ty_int).
+
+Example test_ifThenElse : forall x y,
+  Apply (LamAbs x int_and_int_to_int (Apply (Apply (Var x) (constInt 17)) (constInt 3))) (Apply (TyInst (Apply (LamAbs y Ty_int (Builtin IfThenElse)) (constInt 666)) (Ty_Builtin (Some (TypeIn DefaultUniInteger)))) (Constant (Some (ValueOf DefaultUniBool true)))) ==> constInt 17.
+Proof.
+  intros.
+  eapply E_Apply.
+  - apply E_LamAbs.
+  - eapply E_IfCondition.
+    + eapply E_IfTyInst. 
+      eapply E_Apply.
+      * apply E_LamAbs.
+      * apply E_Constant.
+      * apply S_Builtin.
+      * apply E_Builtin.
+    + apply E_Constant.
+  - apply S_Apply.
+    + apply S_Apply.
+      * apply S_Var1.
+      * apply S_Constant.
+    + apply S_Constant.
+  - eapply E_IfTrue.
+    + apply E_IfThenBranch.
+      * apply E_IfCondition.
+        -- apply E_IfTyInst.
+           apply E_Builtin.
+        -- apply E_Constant.
+    + apply E_Constant.
+Qed.
